Changes suggested by @kyoDralliam

ulib/FStar.ListProperties.fst
@@ -24,6 +24,12 @@ val mem_empty : #a:eqtype -> x:a ->
         (ensures False)
 let mem_empty #a x = ()
 
+val mem_existsb: #a:eqtype -> f:(a -> Tot bool) -> xs:list a ->
+  Lemma(ensures (existsb f xs <==> (exists (x:a). (f x = true /\ mem x xs))))
+let rec mem_existsb #a f xs =
+  match xs with
+  | [] -> ()
+  | hd::tl -> mem_existsb f tl
 
 (** Properties about rev **)
 
@@ -50,6 +56,7 @@ val rev_mem : #a:eqtype -> l:list a -> x:a ->
   Lemma (requires True)
         (ensures (mem x (rev l) <==> mem x l))
 let rev_mem #a l x = rev_acc_mem l [] x
+
 
 (** Properties about append **)
 
@@ -163,16 +170,6 @@ let rec append_inv_tail #a l l1 l2 = match l1, l2 with
        (* Idem *)
        )
 
-(** Properties about flatten **)
-
-val flatten_cons_append: #a:eqtype
-  -> (xs: list a)
-  -> (ys: list a)
-  -> (zzs: list (list a))
-  -> Lemma(ensures
-    (flatten (Cons (append xs ys) zzs) = append xs (append ys (flatten zzs))))
-let flatten_cons_append #a xs ys zzs =
-  append_assoc xs ys (flatten zzs)
 
 (** Properties mixing rev and append **)
 
@@ -218,22 +215,6 @@ val rev_involutive : #a:eqtype -> l:list a ->
         (ensures (rev (rev l) = l))
 let rev_involutive #a l = rev_rev' l; rev_rev' (rev' l); rev'_involutive l
 
-val rev_acc_append:  #t:eqtype -> a:list t -> b:list t -> c:list t ->
-  Lemma(ensures append (rev_acc a b) c = rev_acc a (append b c))
-let rev_acc_append #t a b c =
-  rev_acc_rev' a b;
-  rev_acc_rev' a (append b c);
-  append_assoc (rev' a) b c
-
-(* Seems a little unnatural *)
-val rev_cons: #a:eqtype -> (xs: list a) -> (r: list a) -> (x:a) ->
-  Lemma(requires (xs = rev_acc r []))
-    (ensures (append xs (Cons x []) = rev_acc (Cons x r) []))
-let rev_cons #a xs r x =
-  rev_acc_rev' ([x]@r) [];
-  rev_append [x] r;
-  rev_acc_rev' r [];
-  append_l_nil ((rev' r)@[])
 
 (** Reverse induction principle **)
 
